finalize vlbytes

src/lowparse/LowParse.Low.Bytes.fst
@@ -38,6 +38,17 @@ let valid_flbytes_intro
   ))
 = valid_facts (parse_flbytes sz) h s pos
 
+let valid_pos_flbytes_elim
+  (h: HS.mem)
+  (sz: nat { sz < 4294967296 } )
+  (s: slice)
+  (pos pos' : U32.t)
+: Lemma
+  (requires (valid_pos (parse_flbytes sz) h s pos pos'))
+  (ensures (U32.v pos + sz == U32.v pos'))
+  [SMTPat (valid_pos (parse_flbytes sz) h s pos pos')]
+= valid_facts (parse_flbytes sz) h s pos
+
 let clens_flbytes_slice
   (sz: nat)
   (from: U32.t)
@@ -113,10 +124,9 @@ let accessor_flbytes_get
 
 inline_for_extraction
 let serialize32_flbytes
-  (sz: nat)
-  (sz32: U32.t { U32.v sz32 == sz } )
-: Tot (serializer32 (serialize_flbytes sz))
-= fun (src: BY.lbytes sz) (dst: buffer8) ->
+  (sz32: U32.t)
+: Tot (serializer32 (serialize_flbytes (U32.v sz32)))
+= fun (src: BY.lbytes (U32.v sz32)) (dst: buffer8) ->
   begin if sz32 <> 0ul
   then
     let dst' = B.sub dst 0ul sz32 in
@@ -126,26 +136,23 @@ let serialize32_flbytes
 
 inline_for_extraction
 let write_flbytes
-  (sz: nat)
-  (sz32: U32.t { U32.v sz32 == sz } ) 
-: Tot (leaf_writer_strong (serialize_flbytes sz))
-= leaf_writer_strong_of_serializer32 (serialize32_flbytes sz sz32) ()
+  (sz32: U32.t)
+: Tot (leaf_writer_strong (serialize_flbytes (U32.v sz32)))
+= leaf_writer_strong_of_serializer32 (serialize32_flbytes sz32) ()
 
 inline_for_extraction
 let write_flbytes_weak
-  (sz: nat { sz < 4294967295 } ) // need to return that value if output buffer is too small
-  (sz32: U32.t { U32.v sz32 == sz } ) 
-: Tot (leaf_writer_weak (serialize_flbytes sz))
-= leaf_writer_weak_of_strong_constant_size (write_flbytes sz sz32) sz32 ()
+  (sz32: U32.t { U32.v sz32 < 4294967295 } )  // need to return that value if output buffer is too small
+: Tot (leaf_writer_weak (serialize_flbytes (U32.v sz32)))
+= leaf_writer_weak_of_strong_constant_size (write_flbytes sz32) sz32 ()
 
 inline_for_extraction
 let read_flbytes
-  (sz: nat)
-  (sz32: U32.t { U32.v sz32 == sz } )
-: Tot (leaf_reader (parse_flbytes sz))
+  (sz32: U32.t)
+: Tot (leaf_reader (parse_flbytes (U32.v sz32)))
 = fun input pos ->
   let h = HST.get () in
-  [@inline_let] let _ = valid_facts (parse_flbytes sz) h input pos in
+  [@inline_let] let _ = valid_facts (parse_flbytes (U32.v sz32)) h input pos in
   BY.of_buffer sz32 (B.sub input.base pos sz32)
 
 
@@ -278,8 +285,8 @@ let clens_vlbytes_length
   clens_get = (fun (x: parse_bounded_vlbytes_t min max) -> (x <: Ghost (BY.lbytes length) (requires (clens_vlbytes_length_cond min max length x)) (ensures (fun _ -> True))));
 }
 
-(*
-#reset-options "--z3rlimit 64 --max_fuel 2 --initial_fuel 2 --max_ifuel 6 --initial_ifuel 6 --z3cliopt smt.arith.nl=false"
+
+#push-options "--z3rlimit 16 --max_fuel 2 --initial_fuel 2 --max_ifuel 6 --initial_ifuel 6"
 
 let gaccessor_vlbytes_length
   (min: nat)
@@ -287,27 +294,82 @@ let gaccessor_vlbytes_length
   (length: nat { length < 4294967296 } )
 : Tot (gaccessor (parse_bounded_vlbytes min max) (parse_flbytes length) (clens_vlbytes_length min max length))
 = fun (input: bytes) -> (begin
-    let res = if Seq.length input >= log256' max + length
+    let res = if Seq.length input = log256' max + length
     then (log256' max, length)
     else (0, 0)
     in
     let g () : Lemma
       (requires (gaccessor_pre (parse_bounded_vlbytes min max) (parse_flbytes length) (clens_vlbytes_length min max length) input))
       (ensures (gaccessor_post (parse_bounded_vlbytes min max) (parse_flbytes length) (clens_vlbytes_length min max length) input res))
-    = assert (Some? (parse (parse_bounded_vlbytes min max) input));
-      let (Some (payload_length, consumed_header)) = parse (parse_bounded_integer (log256' max)) input in
-      assert (consumed_header == log256' max);
-      let pos'  = log256' max + U32.v payload_length in
-      assert (pos' <= Seq.length input);
-      let (Some (x, consumed_payload)) = parse parse_all_bytes (Seq.slice input (log256' max) pos') in
-      admit ()
+    = parse_bounded_vlbytes_eq min max input
     in
     Classical.move_requires g ();
     res
   end <: Ghost (nat & nat) (requires True) (ensures (fun res -> gaccessor_post' (parse_bounded_vlbytes min max) (parse_flbytes length) (clens_vlbytes_length min max length) input res)))
 
+#pop-options
 
-admit ()
+#push-options "--z3rlimit 64 --max_fuel 2 --initial_fuel 2 --max_ifuel 6 --initial_ifuel 6"
+
+let valid_bounded_vlbytes_intro
+  (h: HS.mem)
+  (min: nat)
+  (max: nat { min <= max /\ max > 0 /\ max < 4294967296 } )
+  (input: slice)
+  (pos: U32.t)
+  (len: U32.t)
+: Lemma
+  (requires (
+    let sz = log256' max in
+    min <= U32.v len /\ U32.v len <= max /\
+    valid (parse_bounded_integer sz) h input pos /\
+    contents (parse_bounded_integer sz) h input pos == len /\
+    U32.v pos + sz <= 4294967295 /\ (
+    let pos_payload = pos `U32.add` U32.uint_to_t sz in
+    valid (parse_flbytes (U32.v len)) h input pos_payload
+  )))
+  (ensures (
+    let sz = log256' max in  
+    let pos_payload = pos `U32.add` U32.uint_to_t sz in
+    valid_content_pos (parse_bounded_vlbytes min max) h input pos (contents (parse_flbytes (U32.v len)) h input pos_payload) (pos_payload `U32.add` len)
+  ))
+= valid_facts (parse_bounded_vlbytes min max) h input pos;
+  parse_bounded_vlbytes_eq min max (B.as_seq h (B.gsub input.base pos (input.len `U32.sub` pos)));
+  let sz = log256' max in
+  valid_facts (parse_bounded_integer sz) h input pos;
+  valid_facts (parse_flbytes (U32.v len)) h input (pos `U32.add` U32.uint_to_t sz)
+
+#pop-options
+
+inline_for_extraction
+let finalize_bounded_vlbytes
+  (min: nat)
+  (max: nat { min <= max /\ max > 0 /\ max < 4294967296 } )
+  (input: slice)
+  (pos: U32.t)
+  (len: U32.t)
+: HST.Stack U32.t
+  (requires (fun h ->
+    let sz = log256' max in
+    min <= U32.v len /\ U32.v len <= max /\
+    U32.v pos + sz <= 4294967295 /\ (
+    let pos_payload = pos `U32.add` U32.uint_to_t sz in
+    valid (parse_flbytes (U32.v len)) h input pos_payload
+  )))
+  (ensures (fun h pos' h' ->
+    let sz = log256' max in  
+    let pos_payload = pos `U32.add` U32.uint_to_t sz in
+    B.modifies (loc_slice_from_to input pos pos_payload) h h' /\
+    valid_content_pos (parse_bounded_vlbytes min max) h' input pos (contents (parse_flbytes (U32.v len)) h input pos_payload) pos' /\
+    U32.v pos' == U32.v pos_payload + U32.v len
+  ))
+= [@inline_let]
+  let sz = log256' max in
+  let _ = write_bounded_integer sz len input pos in
+  let h = HST.get () in
+  [@inline_let] let _ = valid_bounded_vlbytes_intro h min max input pos len in
+  (pos `U32.add` U32.uint_to_t sz) `U32.add` len
+
 
 (*
 let h = HST.get () in
